\documentclass[]{standalone}
\usepackage[T1]{fontenc}
\usepackage[utf8]{inputenc}
\usepackage{lmodern}
\usepackage[czech]{babel}
\usepackage{prooftrees}

\begin{document}
\begin{prooftree}
{
to prove={\vdash (\neg \psi\rightarrow \neg\varphi) \rightarrow (\varphi\rightarrow\psi)}
}
[{F: (\neg \psi\rightarrow \neg\varphi) \rightarrow (\varphi\rightarrow\psi)}, just=Negace závěru
  [{T: \neg \psi\rightarrow \neg\varphi}, just=$ \rightarrow\mbox{E} $:!r1, name=limp
    [{F: \varphi\rightarrow\psi}, just=$ \rightarrow\mbox{E} $:!r1, name=rimp   
      [{T: \varphi}, just=$ \rightarrow\mbox{E} $:rimp, name=tfi
        [{F: \psi}, just=$ \rightarrow\mbox{E} $:rimp, name=fpsi
          [{F: \neg\psi}, just=$ \rightarrow\mbox{E} $:limp
            [{T: \psi}, just=$ \neg\mbox{E} $:!u, close={:fpsi,!c}]
          ]
          [{T: \neg\varphi}, just=$ \rightarrow\mbox{E} $:limp
            [{F: \varphi}, just=$ \neg\mbox{E} $:!u, close={:tfi,!c}]
          ]
        ]
      ]
    ]
  ]
]
\end{prooftree}
\end{document}
